src/basic/FStarC.Compiler.Util.fsti
@@ -394,4 +394,4 @@ val array_length (s:FStar.ImmutableArray.Base.t 'a) : FStarC.BigInt.t
 val array_index (s:FStar.ImmutableArray.Base.t 'a) (i:FStarC.BigInt.t) : 'a
 
 val putenv : string -> string -> unit
-val execvp : string -> list string -> unit
+val execvp : string -> list string -> unit // will return only on error
