src/fstar/FStarC.OCaml.fsti
@@ -1,0 +1,30 @@
+(*
+   Copyright 2008-2016 Nikhil Swamy and Microsoft Research
+
+   Licensed under the Apache License, Version 2.0 (the "License");
+   you may not use this file except in compliance with the License.
+   You may obtain a copy of the License at
+
+       http://www.apache.org/licenses/LICENSE-2.0
+
+   Unless required by applicable law or agreed to in writing, software
+   distributed under the License is distributed on an "AS IS" BASIS,
+   WITHOUT WARRANTIES OR CONDITIONS OF ANY KIND, either express or implied.
+   See the License for the specific language governing permissions and
+   limitations under the License.
+*)
+module FStarC.OCaml
+
+open FStarC.Compiler.Effect
+
+(* Escape a string for use in a shell command, expecting to be wrapped in SINGLE quotes. *)
+val shellescape (s:string) : string
+
+(* Compute a value for OCAMLPATH taken from the current env + extended with our own library.
+This is NOT escaped. *)
+val new_ocamlpath () : string
+
+(* Run a command with the new OCAMLPATH set. The cmd is usually args[0], in Unix convention.
+This calls execvp, so it will not return if successful. Raises a Failure if the execvp fails.
+It also tries to find the command in the PATH, absolute path is not needed. *)
+val exec_in_ocamlenv (#a:Type) (cmd : string) (args : list string) : a
